zoo_saturn/inf_mpmc_queue_1: Verify [push].

theories/zoo_saturn/inf_mpmc_queue_1.v
@@ -1,5 +1,21 @@
 From zoo Require Import
   prelude.
+From zoo.common Require Import
+  countable
+  function.
+From zoo.iris.base_logic Require Import
+  lib.twins
+  lib.mono_list
+  lib.saved_pred
+  lib.oneshot.
+From zoo.language Require Import
+  notations.
+From zoo.diaframe Require Import
+  diaframe.
+From zoo_std Require Import
+  option
+  optional
+  inf_array.
 From zoo_saturn Require Export
   base
   inf_mpmc_queue_1__code.
@@ -8,8 +24,365 @@ From zoo_saturn Require Import
 From zoo Require Import
   options.
 
+Implicit Types front back : nat.
+Implicit Types l : location.
+Implicit Types t v : val.
+Implicit Types vs hist : list val.
+Implicit Types slots : nat → optional val.
+Implicit Types η : gname.
+Implicit Types ηs : list gname.
+
+Class InfMpmcQueue1G Σ `{zoo_G : !ZooG Σ} := {
+  #[local] inf_mpmc_queue_1_G_inf_array_G :: InfArrayG Σ ;
+  #[local] inf_mpmc_queue_1_G_model_G :: TwinsG Σ (leibnizO (list val)) ;
+  #[local] inf_mpmc_queue_1_G_history_G :: MonoListG Σ val ;
+  #[local] inf_mpmc_queue_1_G_consumers_list_G :: MonoListG Σ gname ;
+  #[local] inf_mpmc_queue_1_G_consumers_pred_G :: SavedPredG Σ val ;
+  #[local] inf_mpmc_queue_1_G_tokens_list_G :: MonoListG Σ gname ;
+  #[local] inf_mpmc_queue_1_G_tokens_state_G :: OneshotG Σ () () ;
+}.
+
+Definition inf_mpmc_queue_1_Σ := #[
+  inf_array_Σ ;
+  twins_Σ (leibnizO (list val)) ;
+  mono_list_Σ val ;
+  mono_list_Σ gname ;
+  saved_pred_Σ val ;
+  mono_list_Σ gname ;
+  oneshot_Σ unit unit
+].
+#[global] Instance subG_inf_mpmc_queue_1_Σ Σ `{zoo_G : !ZooG Σ} :
+  subG inf_mpmc_queue_1_Σ Σ →
+  InfMpmcQueue1G Σ.
+Proof.
+  solve_inG.
+Qed.
+
+Section inf_mpmc_queue_1_G.
+  Context `{inf_mpmc_queue_1_G : InfMpmcQueue1G Σ}.
+
+  Implicit Types Ψ : val → iProp Σ.
+
+  Record metadata := {
+    metadata_data : val ;
+    metadata_model : gname ;
+    metadata_history : gname ;
+    metadata_consumers : gname ;
+    metadata_tokens : gname ;
+  }.
+  Implicit Types γ : metadata.
+
+  #[local] Instance metadata_eq_dec : EqDecision metadata :=
+    ltac:(solve_decision).
+  #[local] Instance metadata_countable :
+    Countable metadata.
+  Proof.
+    solve_countable.
+  Qed.
+
+  #[local] Definition model₁' γ_model vs :=
+    twins_twin1 γ_model (DfracOwn 1) vs.
+  #[local] Definition model₁ γ :=
+    model₁' γ.(metadata_model).
+  #[local] Definition model₂' γ_model vs :=
+    twins_twin2 γ_model vs.
+  #[local] Definition model₂ γ :=
+    model₂' γ.(metadata_model).
+
+  #[local] Definition history_auth' γ_history hist :=
+    mono_list_auth γ_history (DfracOwn 1) hist.
+  #[local] Definition history_auth γ :=
+    history_auth' γ.(metadata_history).
+  #[local] Definition history_at γ i v :=
+    mono_list_at γ.(metadata_history) i v.
+
+  #[local] Definition consumers_auth' γ_consumers i : iProp Σ :=
+    ∃ ηs,
+    mono_list_auth γ_consumers (DfracOwn 1) ηs ∗
+    ⌜length ηs = i⌝.
+  #[local] Definition consumers_auth γ i :=
+    consumers_auth' γ.(metadata_consumers) i.
+  #[local] Definition consumers_at γ i Ψ : iProp Σ :=
+    ∃ η,
+    mono_list_at γ.(metadata_consumers) i η ∗
+    saved_pred η Ψ.
+
+  #[local] Definition tokens_auth' γ_tokens i : iProp Σ :=
+    ∃ ηs,
+    mono_list_auth γ_tokens (DfracOwn 1) ηs ∗
+    ⌜length ηs = i⌝.
+  #[local] Definition tokens_auth γ i :=
+    tokens_auth' γ.(metadata_tokens) i.
+  #[local] Definition tokens_pending γ i : iProp Σ :=
+    ∃ η,
+    mono_list_at γ.(metadata_tokens) i η ∗
+    oneshot_pending η (DfracOwn 1) ().
+  #[local] Definition tokens_done γ i : iProp Σ :=
+    ∃ η,
+    mono_list_at γ.(metadata_tokens) i η ∗
+    oneshot_shot η ().
+
+  #[local] Definition consumer_au γ ι Ψ : iProp Σ :=
+    AU <{
+      ∃∃ vs,
+      model₁ γ vs
+    }> @ ⊤ ∖ ↑ι, ∅ <{
+      ∀∀ v vs',
+      ⌜vs = v :: vs'⌝ ∗
+      model₁ γ vs'
+    , COMM
+      Ψ v
+    }>.
+
+  #[local] Definition inv_inner l γ ι : iProp Σ :=
+    ∃ front back hist slots,
+    l.[front] ↦ #front ∗
+    l.[back] ↦ #back ∗
+    inf_array_model γ.(metadata_data) (optional_to_val ∘ slots) ∗
+    history_auth γ hist ∗
+    ⌜length hist = back⌝ ∗
+    model₂ γ (drop front hist) ∗
+    consumers_auth γ front ∗
+    tokens_auth γ (front `max` back) ∗
+    ( [∗ list] i ∈ seq 0 back,
+        tokens_pending γ i
+      ∨ ∃ Ψ v,
+        consumers_at γ i Ψ ∗
+        history_at γ i v ∗
+        Ψ v
+    ) ∗
+    ( [∗ list] i ∈ seq back (front - back),
+      ∃ Ψ,
+      consumers_at γ i Ψ ∗
+      consumer_au γ ι Ψ
+    ) ∗
+    ( ∀ i,
+      match slots i with
+      | Something v =>
+          history_at γ i v
+      | Anything =>
+          tokens_done γ i
+      | Nothing =>
+          True
+      end
+    ).
+  #[local] Instance : CustomIpatFormat "inv_inner" :=
+    "(
+      %front{} &
+      %back{} &
+      %hist{} &
+      %slots{} &
+      Hl_front &
+      Hl_back &
+      >Hdata_model &
+      Hhistory_auth &
+      >%Hhist{} &
+      Hmodel₂ &
+      Hconsumers_auth &
+      Htokens_auth &
+      Hpast &
+      Hwaiters &
+      Hslots
+    )".
+  Definition inf_mpmc_queue_1_inv t ι : iProp Σ :=
+    ∃ l γ,
+    ⌜t = #l⌝ ∗
+    meta l nroot γ ∗
+    l.[data] ↦□ γ.(metadata_data) ∗
+    inf_array_inv γ.(metadata_data) ∗
+    inv ι (inv_inner l γ ι).
+  #[local] Instance : CustomIpatFormat "inv" :=
+    "(
+      %l &
+      %γ &
+      -> &
+      #Hmeta &
+      #Hl_data &
+      #Hdata_inv &
+      #Hinv
+    )".
+
+  Definition inf_mpmc_queue_1_model t vs : iProp Σ :=
+    ∃ l γ,
+    ⌜t = #l⌝ ∗
+    meta l nroot γ ∗
+    model₁ γ vs.
+  #[local] Instance : CustomIpatFormat "model" :=
+    "(
+      %_l &
+      %_γ &
+      %Heq &
+      _Hmeta &
+      Hmodel₁
+    )".
+
+  #[global] Instance inf_mpmc_queue_1_model_timeless t vs :
+    Timeless (inf_mpmc_queue_1_model t vs).
+  Proof.
+    apply _.
+  Qed.
+  #[local] Instance consumers_at_persistent γ i Ψ :
+    Persistent (consumers_at γ i Ψ).
+  Proof.
+    apply _.
+  Qed.
+  #[global] Instance inf_mpmc_queue_1_inv_persistent t ι :
+    Persistent (inf_mpmc_queue_1_inv t ι).
+  Proof.
+    apply _.
+  Qed.
+
+  #[local] Lemma model_agree γ vs1 vs2 :
+    model₁ γ vs1 -∗
+    model₂ γ vs2 -∗
+    ⌜vs1 = vs2⌝.
+  Proof.
+    apply: twins_agree_L.
+  Qed.
+  #[local] Lemma model_update {γ vs1 vs2} vs :
+    model₁ γ vs1 -∗
+    model₂ γ vs2 ==∗
+      model₁ γ vs ∗
+      model₂ γ vs.
+  Proof.
+    apply twins_update'.
+  Qed.
+
+  #[local] Lemma history_update {γ hist} v :
+    history_auth γ hist ⊢ |==>
+      history_auth γ (hist ++ [v]) ∗
+      history_at γ (length hist) v.
+  Proof.
+    iIntros "Hhistory_auth".
+    iMod (mono_list_update_snoc v with "Hhistory_auth") as "Hhistory_auth".
+    iDestruct (mono_list_at_get with "Hhistory_auth") as "#Hhistory_at".
+    { rewrite list_lookup_middle //. }
+    iSteps.
+  Qed.
+
+  #[local] Lemma tokens_update {γ} i :
+    tokens_auth γ i ⊢ |==>
+      tokens_auth γ (S i) ∗
+      tokens_pending γ i.
+  Proof.
+    iIntros "(%ηs & Hauth & %Hηs)".
+    iMod oneshot_alloc as "(%η & Hpending)".
+    iMod (mono_list_update_snoc with "Hauth") as "Hauth".
+    iDestruct (mono_list_at_get with "Hauth") as "#Hat".
+    { rewrite list_lookup_middle //. }
+    iFrame. rewrite length_app. iSteps.
+  Qed.
+
+  Opaque consumers_auth'.
+  Opaque consumers_at.
+  Opaque tokens_auth'.
+  Opaque tokens_pending.
+  Opaque tokens_done.
+
+  Lemma inf_mpmc_queue_1_push_spec t ι v :
+    <<<
+      inf_mpmc_queue_1_inv t ι
+    | ∀∀ vs,
+      inf_mpmc_queue_1_model t vs
+    >>>
+      inf_mpmc_queue_1_push t v @ ↑ι
+    <<<
+      inf_mpmc_queue_1_model t (vs ++ [v])
+    | RET ();
+      True
+    >>>.
+  Proof.
+    iIntros "!> %Φ (:inv) HΦ".
+
+    wp_rec. wp_pures.
+
+    wp_bind (FAA _ _).
+    wp_apply (wp_wand _ _
+      ( λ res,
+        ∃ back,
+        ⌜res = #back⌝ ∗
+        history_at γ back v ∗
+        Φ ()%V
+      )%I
+      with "[HΦ]"
+    ) as (res) "(%back & -> & #Hhistory_at & HΦ)".
+    { iInv "Hinv" as "(:inv_inner =1)".
+      wp_faa.
+
+      iMod (history_update v with "Hhistory_auth") as "(History_auth & #Hhistory_at)".
+      iEval (rewrite Hhist1) in "Hhistory_at".
+
+      iMod "HΦ" as "(%vs & (:model) & _ & HΦ)". injection Heq as <-.
+      iDestruct (meta_agree with "Hmeta _Hmeta") as %<-. iClear "_Hmeta".
+      iDestruct (model_agree with "Hmodel₁ Hmodel₂") as %Hvs.
+      iMod (model_update (vs ++ [v]) with "Hmodel₁ Hmodel₂") as "(Hmodel₁ & Hmodel₂)".
+      iMod ("HΦ" with "[Hmodel₁] [//]") as "$"; first iSteps.
+
+      destruct (decide (front1 ≤ back1)) as [Hback1 | Hback1].
+
+      - rewrite Nat.max_r //.
+
+        iMod (tokens_update with "Htokens_auth") as "(Htokens_auth & Htokens_at)".
+        iDestruct (big_sepL_snoc with "[$Hpast $Htokens_at]") as "Hpast".
+        rewrite -seq_S.
+
+        iSplitL.
+        { iExists front1, (S back1). iFrame.
+          rewrite length_app /=.
+          rewrite Hvs drop_app_le; first lia.
+          rewrite Nat.max_r; first lia.
+          assert (front1 - S back1 = 0) as -> by lia.
+          iSteps.
+        }
+        iSteps.
+
+      - rewrite Nat.max_l; first lia.
+        rewrite (nil_length_inv vs).
+        { rewrite Hvs length_drop. lia. }
+        assert (front1 - back1 = S (front1 - S back1)) as ->; first lia.
+        destruct (Nat.lt_exists_pred 0 (front1 - back1)) as (δ & ? & _); first lia.
+        rewrite -cons_seq. iDestruct "Hwaiters" as "((%Ψ & #Hconsumers_at & HΨ) & Hwaiters)".
+
+        iMod "HΨ" as "(% & Hmodel₁ & _ & HΨ)".
+        iDestruct (model_agree with "Hmodel₁ Hmodel₂") as %->.
+        iMod (model_update [] with "Hmodel₁ Hmodel₂") as "(Hmodel₁ & Hmodel₂)".
+        iMod ("HΨ" with "[$Hmodel₁ //]") as "HΨ".
+
+        iDestruct (big_sepL_snoc with "[$Hpast HΨ]") as "Hpast"; first iSteps.
+        rewrite -seq_S.
+
+        iSplitL.
+        { iFrame.
+          rewrite skipn_all2 length_app /=; first lia.
+          rewrite Nat.max_l; first lia.
+          iSteps.
+        }
+        iSteps.
+    }
+
+    wp_load.
+
+    awp_apply (inf_array_set_spec with "Hdata_inv") without "HΦ"; first lia.
+    iInv "Hinv" as "(:inv_inner =2)".
+    iAaccIntro with "Hdata_model".
+    { iIntros. iFrame. done. }
+    iIntros "Hdata_model !>".
+    iSplitL.
+    { repeat iExists _.
+      rewrite Nat2Z.id -(fn_compose_insert _ _ _ (Something v)).
+      iSteps.
+      rewrite function.fn_lookup_insert.
+      case_decide; first subst; iSteps.
+    }
+    iSteps.
+  Qed.
+End inf_mpmc_queue_1_G.
+
 #[global] Opaque inf_mpmc_queue_1_create.
 #[global] Opaque inf_mpmc_queue_1_size.
 #[global] Opaque inf_mpmc_queue_1_is_empty.
 #[global] Opaque inf_mpmc_queue_1_push.
 #[global] Opaque inf_mpmc_queue_1_pop.
+
+#[global] Opaque inf_mpmc_queue_1_inv.
+#[global] Opaque inf_mpmc_queue_1_model.
